SN_CC.v
@@ -288,11 +288,8 @@ Module SN := GenModelSN.MakeModel SN_CC_Model SN_CC_addon.
 
 (** ** Extendability *)
 Definition cst (x:set) : SN.T.term.
-left; exists (fun _ =>x) (fun _ =>Lambda.K).
+left; exists (fun _ =>x);[|exact Lambda.K].
  do 2 red; reflexivity.
- do 2 red; reflexivity.
- red; reflexivity.
- red; reflexivity.
 Defined.
 
 Definition mkSET (x:set) := cst (mkTY x snSAT).
@@ -411,14 +408,15 @@ Lemma int_lift_rec : forall n t k,
   eq_term (lift_rec n k (int_term t)) (int_term (Tm.lift_rec n t k)).
 induction t; simpl int_term; intros.
  destruct s; simpl; trivial.
- split; red; intros; reflexivity.
+ split; trivial.
+ red; intros; reflexivity.
 
  simpl; unfold V.lams, I.lams, V.shift, I.shift.
  destruct (le_gt_dec k n0); simpl.
   replace (k+(n+(n0-k))) with (n+n0) by omega.
-  split; red; auto.
+  split; [red|]; auto.
 
-  split; red; auto.
+  split; [red|]; auto.
 
  rewrite red_lift_abs; rewrite IHt1; rewrite IHt2; reflexivity.
  rewrite red_lift_app; rewrite IHt1; rewrite IHt2; reflexivity.
@@ -440,7 +438,7 @@ Lemma int_subst_rec : forall arg,
 intros arg not_knd.
 induction t; simpl int_term; intros.
  destruct s; simpl; trivial.
- split; red; intros; reflexivity.
+ split; [red|]; intros; reflexivity.
 
  simpl Tm.subst_rec.
  destruct (lt_eq_lt_dec k n) as [[fv|eqv]|bv]; simpl int_term.
