SN_ECC.v
@@ -162,11 +162,8 @@ Module SN := GenModelSN.MakeModel SN_ECC_Model SN_ECC_addon.
 
 (** ** Extendability *)
 Definition cst (x:set) : SN.T.term.
-left; exists (fun _ =>x) (fun _ =>Lambda.K).
+left; exists (fun _ =>x);[|exact Lambda.K].
  do 2 red; reflexivity.
- do 2 red; reflexivity.
- red; reflexivity.
- red; reflexivity.
 Defined.
 
 Definition mkSET (x:set) := cst (mkTY x snSAT).
@@ -356,6 +353,7 @@ split.
   unfold SN_ECC_addon.Real in *; simpl SN.T.int in *.
   rewrite Real_sort_sn in *.
   simpl in satU|-*.
+  rewrite <- !SN.T.tm_tmm.
   rewrite SN.T.tm_subst_cons in satU.
   apply sat_sn in satU.
   apply Lambda.sn_subst in satU.
@@ -400,16 +398,16 @@ Lemma int_lift_rec : forall n t k,
   eq_term (lift_rec n k (int_term t)) (int_term (Tm.lift_rec n t k)).
 induction t; simpl int_term; intros.
  destruct s; simpl; trivial.
- split; red; intros; reflexivity.
+ split; [red|]; intros; reflexivity.
 
- split; red; intros; reflexivity.
+ split; [red|]; intros; reflexivity.
 
  simpl; unfold V.lams, I.lams, V.shift, I.shift.
  destruct (le_gt_dec k n0); simpl.
   replace (k+(n+(n0-k))) with (n+n0) by omega.
-  split; red; auto.
+  split; [red|]; auto.
 
-  split; red; auto.
+  split; [red|]; auto.
 
  rewrite red_lift_abs; rewrite IHt1; rewrite IHt2; reflexivity.
  rewrite red_lift_app; rewrite IHt1; rewrite IHt2; reflexivity.
@@ -431,9 +429,9 @@ Lemma int_subst_rec : forall arg,
 intros arg not_knd.
 induction t; simpl int_term; intros.
  destruct s; simpl; trivial.
- split; red; intros; reflexivity.
+ split; [red|]; intros; reflexivity.
 
- split; red; intros; reflexivity.
+ split; [red|]; intros; reflexivity.
 
  simpl Tm.subst_rec.
  destruct (lt_eq_lt_dec k n) as [[fv|eqv]|bv]; simpl int_term.
